VisualProof/Rule/Step.lean
@@ -2,7 +2,6 @@ import VisualProof.Rule.Erasure
 import VisualProof.Rule.WireSever
 import VisualProof.Rule.Iteration
 import VisualProof.Rule.DoubleCut
-import VisualProof.Rule.Comprehension.Relation
 import VisualProof.Rule.Vacuity
 
 namespace VisualProof.Rule
@@ -14,7 +13,6 @@ inductive Step : OpenDiagram arity → OpenDiagram arity → Prop
   | wireSever : WireSever source target → Step source target
   | iteration : Iteration source target → Step source target
   | doubleCut : DoubleCut source target → Step source target
-  | comprehension : Comprehension source target → Step source target
   | vacuity : Vacuity source target → Step source target
 
 theorem Step.iso
@@ -33,8 +31,6 @@ theorem Step.iso
       exact .iteration (Iteration.iso sourceIso step targetIso)
   | doubleCut step =>
       exact .doubleCut (DoubleCut.iso sourceIso step targetIso)
-  | comprehension step =>
-      exact .comprehension (Comprehension.iso sourceIso step targetIso)
   | vacuity step =>
       exact .vacuity (Vacuity.iso sourceIso step targetIso)
 
